@prefix sws: <http://vocab.inf.ed.ac.uk/sws/a1546360/sws> .
@prefix owl: <http://www.w3.org/2002/07/owl#> .
@prefix xsd: <http://www.w3.org/2001/XMLSchema#> .
@prefix rdfs: <http://www.w3.org/2000/01/rdf-schema#> .
@prefix org: <http://www.w3.org/ns/org#> .
@prefix skos: <http://www.w3.org/2004/02/skos/core#> .
@prefix db: <http://dbpedia.org/resource/classes#> .

sws:response a rdf:Property ;
  skos:prefLabel "Response"@en ;
  skos:altLabel "nameOrTypeOfResponse"@en ;
  rdfs:comment "A property used to give information about the delivered response type."@en .

sws:capacity a rdf:Property ;
  skos:prefLabel "Capacity"@en;
  rdfs:comment "A property used to give information about the amount or type of the resources the organization was able to provide."@en .

sws:NgoInternational a skos:Concept ;
  skos:prefLabel "NGO - International"@en;
  owl:sameAs <http://dbpedia.org/resource/International_NGO>;
  rdfs:comment "Concept of an international Non Governmental Organization"@en .

sws:NgoLocal a skos:Concept ;
  skos:prefLabel "NGO - Local"@en;
  skos:broader <http://dbpedia.org/resource/Non-governmental_organization>;
  rdfs:comment "Concept of a local Non Governmental Organization."@en .

sws:Government a skos:Concept ;
  skos:prefLabel "Government"@en;
  rdfs:comment "Concept of a Governmental Organization."@en .

sws:Corporation a skos:Concept ;
  skos:prefLabel "Corporation"@en;
  rdfs:comment "Concept of a Corporation Organization."@en .

sws:DevelopmentBank a skos:Concept ;
  skos:prefLabel "Development Bank"@en;
  skos:broader <http://dbpedia.org/resource/Bank>;
  rdfs:comment "Concept of a Development Bank Organization."@en .

sws:PoliticalParty a skos:Concept ;
  skos:prefLabel "Political Party"@en;
  owl:sameAs <http://dbpedia.org/resource/Political_party>;
  rdfs:comment "Concept of a Political Party Organization."@en .

sws:Individuals a skos:Concept ;
  skos:prefLabel "Individuals"@en;
    rdfs:comment "Concept of Individuals."@en .

sws:UNAgency a skos:Concept ;
  skos:prefLabel "UN Agency"@en;
  skos:related <http://dbpedia.org/resource/Category:United_Nations_specialized_agencies>;
  rdfs:comment "Concept of a UN Agency as an organization."@en .

sws:organizationTypes a skos:Collection;
  skos:prefLabel "Organization types"@en;
  skos:member sws:NgoInternational;
  skos:member sws:NgoLocal;
  skos:member sws:Government;
  skos:member sws:Corporation;
  skos:member sws:DevelopmentBank;
  skos:member sws:PoliticalParty;
  skos:member sws:Individuals;
  skos:member sws:UNAgency.

sws:donationLink a rdf:Property ;
  skos:prefLabel "Donation Link"@en;
  rdfs:comment "Concept of a link where donations can be made for the associated organization."@en .

sws:newsAndSourceLink a rdf:Property ;
  skos:prefLabel "News And Source Link"@en;
  rdfs:comment "Concept of a link where news can be found about the associated organization."@en .

sws:Nutrition a skos:Concept ;
  skos:prefLabel "Nutrition"@en;
  skos:related <http://dbpedia.org/resource/Nutrition> ;
  rdfs:comment "Concept used to classify an organization that responded in the field of nutrition to a disaster incident."@en .

sws:EarlyRecovery a skos:Concept ;
  skos:prefLabel "Early Recovery"@en;
  rdfs:comment "Concept used to classify an organization that responded in the field of early recovery to a disaster incident."@en .

sws:ShelterAndNFI a skos:Concept ;
  skos:prefLabel "Shelter And NFI"@en;
  rdfs:comment "Concept used to classify an organization that responded in the field of shelter and NFI to a disaster incident."@en .

sws:SearchAndRescue a skos:Concept ;
  skos:prefLabel "Search And Rescue"@en;
  owl:sameAs <http://dbpedia.org/resource/Search_and_rescue> ;
  rdfs:comment "Concept used to classify an organization that responded in the field of search and rescue to a disaster incident."@en .

sws:Wash a skos:Concept ;
  skos:prefLabel "Wash"@en;
  rdfs:comment "Concept used to classify an organization that responded in the field of wash to a disaster incident."@en .

sws:Logistics a skos:Concept ;
  skos:prefLabel "Logistics"@en;
  owl:sameAs <http://dbpedia.org/resource/Logistics> ;
  rdfs:comment "Concept used to classify an organization that responded in the field of logistics to a disaster incident."@en .

sws:Telecom a skos:Concept ;
  skos:prefLabel "Telecom"@en;
  skos:related <http://dbpedia.org/resource/Telecommunication> ;
  rdfs:comment "Concept used to classify an organization that responded in the field of telecom to a disaster incident."@en .

sws:Health a skos:Concept ;
  skos:prefLabel "Health"@en;
  rdfs:comment "Concept used to classify an organization that responded in the field of health to a disaster incident."@en .

sws:Assessments a skos:Concept ;
  skos:prefLabel "Assessments"@en;
  rdfs:comment "Concept used to classify an organization that responded in the field of assessments to a disaster incident."@en .

sws:Funding a skos:Concept ;
  skos:prefLabel "Funding"@en;
  skos:related <http://dbpedia.org/resource/Fundraising> ;
  rdfs:comment "Concept used to classify an organization that responded in the field of funding to a disaster incident."@en .

sws:Protection a skos:Concept ;
  skos:prefLabel "Protection"@en;
  rdfs:comment "Concept used to classify an organization that responded in the field of protection to a disaster incident."@en .

sws:Education a skos:Concept ;
  skos:prefLabel "Education"@en;
  skos:related <http://dbpedia.org/resource/Education> ;
  rdfs:comment "Concept used to classify an organization that responded in the field of education to a disaster incident."@en .

sws:FoodSecurity a skos:Concept ;
  skos:prefLabel "Food Security"@en;
  owl:sameAs <http://dbpedia.org/resource/Food_security> ;
  rdfs:comment "Concept used to classify an organization that responded in the field of food security to a disaster incident."@en .

sws:CampCoordination a skos:Concept ;
  skos:prefLabel "Camp Coordination"@en;
  rdfs:comment "Concept used to classify an organization that responded in the field of camp coordination to a disaster incident."@en .

sws:AnimalRescue a skos:Concept ;
  skos:prefLabel "Animal Rescue"@en;
  rdfs:comment "Concept used to classify an organization that responded in the field of animal rescue to a disaster incident."@en .

sws:responseTypes a skos:Collection;
  skos:prefLabel "Response Type"@en;
  rdfs:comment "Collection used to classify organizations in regard to their response to disaster incidents."@en;
  skos:member sws:Nutrition;
  skos:member sws:EarlyRecovery;
  skos:member sws:ShelterAndNFI;
  skos:member sws:SearchAndRescue;
  skos:member sws:Wash;
  skos:member sws:Logistics;
  skos:member sws:Telecom;
  skos:member sws:Health;
  skos:member sws:Assessments;
  skos:member sws:Funding;
  skos:member sws:Protection;
  skos:member sws:Education;
  skos:member sws:FoodSecurity;
  skos:member sws:CampCoordination .






